core/properties/surjectivity/Moore2Mealy_surjectivity_model_witness.v
@@ -1,0 +1,64 @@
+Require Import String.
+Require Import List.
+Require Import Multiset.
+Require Import ListSet.
+
+Require Import core.utils.Utils.
+
+Require Import core.modeling.ConcreteSyntax.
+Require Import core.modeling.ModelingSemantics.
+Require Import core.modeling.ModelingMetamodel.
+Require Import core.modeling.ConcreteExpressions.
+Require Import core.modeling.Parser.
+
+Require Import transformations.Moore2Mealy.Moore.
+Require Import transformations.Moore2Mealy.Mealy.
+Require Import transformations.Moore2Mealy.MooreSemantics.
+
+
+Require Import core.TransformationConfiguration.
+Require Import core.modeling.ModelingTransformationConfiguration.
+
+#[export]
+Instance Moore2MealyTransformationConfiguration : TransformationConfiguration := 
+  Build_TransformationConfiguration Moore.MM Mealy.MM.
+
+#[export]  
+Instance Moore2MealyModelingTransformationConfiguration : ModelingTransformationConfiguration Moore2MealyTransformationConfiguration :=
+ Build_ModelingTransformationConfiguration Moore2MealyTransformationConfiguration Moore.MMM Mealy.MMM.
+
+Open Scope coqtl.
+
+Import Glue.
+Import Nat.
+
+Import Moore.
+
+Definition convert_state : Mealy.State_t :=
+  {| Mealy.State_id := (Id.Id "S0") |}.
+
+(** a transformation that always generate the same element *)
+
+Definition Moore2Mealy' :=
+    transformation
+    [     
+      rule "state"
+      from [State_K]
+      to [
+        ELEM "s" ::: Mealy.State_K  
+           fun _ _ s => return convert_state 
+      ];
+      
+      rule "transition"
+      from [Transition_K]
+      to [
+        ELEM "t" ::: Mealy.State_K
+          fun _ _ s => return convert_state 
+      ]
+].
+    
+Definition Moore2Mealy := parse Moore2Mealy'.
+
+Close Scope coqtl.
+
+  
